Rec call rule experimentation

coq-osiris/theories/proofmode/capital_SIMP.v
@@ -2,6 +2,7 @@ From osiris Require Import base.
 From osiris.lang Require Import lang.
 From osiris.semantics Require Import semantics.
 From osiris.proofmode Require Import equality simp.
+From osiris.proofmode Require Import notations.
 
 (* This file also defines the judgement [SIMP m φ], which asserts that the
    computation [m] is pure and eventually produces a result that satisfies
@@ -326,6 +327,22 @@ Proof.
   done.
 Qed.
 
+Lemma SIMP_Eval `{Encode X} η e k ko (φ : X -> Prop) :
+  SIMP (try (eval η e) k ko) φ ->
+  SIMP (Stop CEval (η, e) k ko) φ.
+Proof.
+  intros.
+  by eapply SIMP_simp; first apply SimpEval.
+Qed.
+
+Lemma SIMP_EvalRetNext `{Encode X} η e (φ : X -> Prop) :
+  SIMP (eval η e) φ ->
+  SIMP (Stop CEval (η, e) ret (fun _ => Next)) φ.
+Proof.
+  intros.
+  by eapply SIMP_simp; [apply advance_SimpEvalRetNext; apply SimpReflexive|].
+Qed.
+
 (* Todo: write comment *)
 
 Lemma SIMP_rec_call `{Encode X} `{Encode Y}
@@ -342,11 +359,13 @@ Lemma SIMP_rec_call `{Encode X} `{Encode Y}
       SIMP (let δ := concat (eval_rec_bindings η rbs) η in
             let η := replace_env_binding δ fname vf in
             'afun ← lookup_rec_bindings rbs fname ;
-            acall η afun #v'
+            let 'AnonFun x e := afun in
+            let η0 := EnvCons x #v' η in
+            eval η0 e
         ) (φ v')) ->
   SIMP (call (VCloRec η rbs fname) #v) (φ v).
 Proof.
-  intros Hwf HP Hrec.
+  intros Hwf HP Hrec. 
   induction v as [v IH] using (well_founded_induction Hwf); intros.
   apply SIMP_enter_call_VCloRec; simpl in *.
   destruct (lookup_rec_bindings_cases rbs fname) as [Hlkp|[afun Hlkp]].
@@ -355,11 +374,174 @@ Proof.
   { specialize (Hrec (VCloRec η rbs fname) v HP).
     rewrite Hlkp in *; simpl in *.
     erewrite replace_binding_idempotent in Hrec by apply Hlkp.
+    unfold acall; destruct afun; apply SIMP_EvalRetNext.
     eapply Hrec; auto.
     intros. rewrite Hlkp. by apply IH. }
 Qed.
 
+Notation "fname 'to' afun" :=
+  (RecBinding fname afun) (at level 50).
 
+Notation "'RecBind' x" := (RecBiCons x RecBiNil) (at level 70). 
+
+Notation "'RecBinds' x ; y ; .. ; z" :=
+  (RecBiCons x (RecBiCons y .. (RecBiCons z RecBiNil) ..))
+    (at level 60,
+      format "'RecBinds'  x ;  '/' y ; '/' .. ; '/' z").
+
+Lemma SIMP_rec_call_unary `{Encode X} `{Encode Y}
+  (η : env) afun (fname : var) (v : X)
+  (P : X -> Prop) (φ : X -> Y -> Prop) (R : X -> X -> Prop) :
+  well_founded R ->
+  P v ->
+  (forall (vf : val) v',
+      P v' ->
+      (forall v'',
+          P v'' ->
+          R v'' v' ->
+          SIMP (call vf #v'') (φ v'')) -> 
+      SIMP (let 'AnonFun x e := afun in
+            eval (EnvCons x #v' (EnvCons fname vf η)) e) (φ v')) ->
+  SIMP (call (VCloRec η (RecBind fname to afun) fname) #v) (φ v).
+Proof.
+  intros Hwf HP Hrec.
+  induction v as [v IH] using (well_founded_induction Hwf); intros.
+  apply SIMP_enter_call_VCloRec; simpl; rewrite String.eqb_refl.
+  unfold acall; destruct afun; apply SIMP_EvalRetNext.
+  eapply Hrec; auto.
+Qed.
+
+Lemma SIMP_rec_call_binary_mutual `{Encode X} `{Encode Y}
+  (η : env) (afun agun : anonfun) (gname fname : var) (v : X)
+  (P : X -> Prop) (φ : X -> Y -> Prop) (R : X -> X -> Prop) :
+  well_founded R ->
+  P v ->
+  (forall (vf : val) v',
+      P v' ->
+      (forall v'',
+          P v'' ->
+          R v'' v' ->
+          SIMP (call vf #v'') (φ v'')) -> 
+      SIMP (let 'AnonFun x e := afun in
+            eval (x ~> #v';
+                  fname ~> vf;
+                  gname ~> (VCloRec η (RecBinds fname to afun; gname to agun) gname);
+                  η) e) (φ v')) ->
+  SIMP (call (VCloRec η (RecBinds fname to afun; gname to agun) fname) #v) (φ v).
+Proof.
+  intros Hwf HP Hrec.
+  induction v as [v IH] using (well_founded_induction Hwf); intros.
+  apply SIMP_enter_call_VCloRec; simpl; rewrite String.eqb_refl.
+  unfold acall; destruct afun; apply SIMP_EvalRetNext.
+  eapply Hrec; auto.
+Qed.
+
+Lemma SIMP_rec_call_binary_mutual_aliasing `{Encode X} `{Encode Y}
+  (η : env) ef eg farg garg (gname fname : var) (v : X)
+  (P : X -> Prop) (φ : X -> Y -> Prop) (R : X -> X -> Prop) :
+  well_founded R ->
+  P v ->
+  (forall (vf : val) v',
+      P v' ->
+      (forall v'',
+          P v'' ->
+          R v'' v' ->
+          SIMP (call vf #v'') (φ v'')) -> 
+      SIMP (eval ((if (fname =? gname)%string then garg else farg) ~> #v';
+                  gname ~>
+                    if (fname =? gname)%string
+                    then vf
+                    else (VCloRec
+                            η
+                            (RecBinds
+                               gname to (AnonFun garg eg);
+                             fname to (AnonFun farg ef))
+                            gname);
+                  fname ~> vf;
+                  η) (if (fname =? gname)%string then eg else ef)) (φ v')) ->
+  SIMP (call (VCloRec η (RecBinds gname to (AnonFun garg eg); fname to (AnonFun farg ef)) fname) #v) (φ v).
+Proof.
+  intros Hwf HP Hrec.
+  induction v as [v IH] using (well_founded_induction Hwf); intros.
+  apply SIMP_enter_call_VCloRec; simpl; rewrite String.eqb_refl.
+  unfold acall; destruct (fname =? gname)%string eqn:name_eq; apply SIMP_EvalRetNext.
+  { apply String.eqb_eq in name_eq as ->. eapply Hrec; eauto. }
+  eapply Hrec; eauto.
+Qed.
+
+Lemma SIMP_rec_call_binary_mutual2 `{Encode X} `{Encode Y}
+  (η : env) ef farg agun (gname fname : var) (v : X)
+  (P : X -> Prop) (φ : X -> Y -> Prop) (R : X -> X -> Prop) :
+  well_founded R ->
+  P v ->
+  (fname =? gname)%string = false ->
+  (forall (vf : val) v',
+      P v' ->
+      (forall v'',
+          P v'' ->
+          R v'' v' ->
+          SIMP (call vf #v'') (φ v'')) -> 
+      SIMP (eval (farg ~> #v';
+                  gname ~>
+                    (VCloRec η (RecBinds gname to agun; fname to (AnonFun farg ef)) gname);
+                  fname ~> vf;
+                  η) ef) (φ v')) ->
+  SIMP (call (VCloRec η (RecBinds gname to agun; fname to (AnonFun farg ef)) fname) #v) (φ v).
+Proof.
+  intros Hwf HP Hname Hrec.
+  induction v as [v IH] using (well_founded_induction Hwf); intros.
+  apply SIMP_enter_call_VCloRec; simpl; rewrite String.eqb_refl.
+  unfold acall; rewrite Hname; apply SIMP_EvalRetNext.
+  eapply Hrec; eauto.
+Qed.
+
+Definition nested_SIMP `{Encode X} vf arg1 arg2 (φ : X -> Prop) :=
+  SIMP (call vf arg1) (fun c =>
+                         SIMP (call c arg2) φ).
+
+Lemma SIMP_nested_rec_call `{Encode A} `{Encode B} `{Encode C}
+  (η : env) farg farg2 ef ef2 (fname : var) (v1 : A) (v2 : B)
+  (P : A -> B -> Prop) (φ : A -> B -> C -> Prop) (R : (A * B) -> (A * B) -> Prop) :
+  let vclo := (VCloRec η (RecBind fname to (AnonFun farg ef)) fname) in
+  well_founded R ->
+  P v1 v2 ->
+  let η1 := (farg ~> #v1; fname ~> vclo; η) in
+  eval η1 ef = ret (VClo η1 (AnonFun farg2 ef2)) ->
+  (forall (vf : val) v1' v2',
+      P v1' v2' ->
+      (forall v1'' v2'',
+          let η1' := (farg ~> #v1''; fname ~> vclo; η) in
+          eval η1' ef = ret (VClo η1' (AnonFun farg2 ef2)) ->
+          P v1'' v2'' ->
+          R (v1'', v2'') (v1', v2') ->
+          nested_SIMP vf #v1'' #v2'' (φ v1'' v2'')) ->
+      let δ := (farg2 ~> #v2'; farg ~> #v1'; fname ~> vf; η) in
+      SIMP (eval δ ef2) (φ v1' v2')) ->
+  nested_SIMP vclo #v1 #v2 (φ v1 v2).
+Proof.
+  cbn zeta.
+  intros Hwf HP Heval Hrec.
+  remember (v1, v2) as p eqn:Hpeq.
+  replace v1 with (p.1) in * by (rewrite Hpeq; reflexivity).
+  replace v2 with (p.2) in * by (rewrite Hpeq; reflexivity).
+  clear v1 v2 Hpeq.
+  induction p as [p IH] using (well_founded_induction Hwf); intros.
+  destruct p as [v1 v2]; simpl in *.
+  apply SIMP_enter_call_VCloRec; simpl; rewrite String.eqb_refl; simpl.
+  
+  unfold acall; apply SIMP_EvalRetNext.
+  rewrite Heval. eapply SIMP_ret; first solve [encode].
+  apply SIMP_enter_call_VClo; simpl; apply SIMP_EvalRetNext.
+  eapply Hrec; auto; intros.
+  apply (IH (v1'', v2'')); auto.
+Qed.
+
+
+
+
+
+
+  
 (* -------------------------------------------------------------------------- *)
 
 (* Tactics. *)
